thys/MFODL_Monitor_Devel/Optimized_Trigger.thy
@@ -17,13 +17,22 @@ type_synonym 'a mtaux = "(ts \<times> 'a table \<times> 'a table) list"
 definition init_targs :: "\<I> \<Rightarrow> nat \<Rightarrow> nat set \<Rightarrow> nat set \<Rightarrow> targs" where
   "init_targs I n L R = \<lparr>targs_ivl = I, targs_n = n, targs_L = L, targs_R = R\<rparr>"
 
-definition trigger_results :: "\<I> \<Rightarrow> ts \<Rightarrow> 'a mtaux \<Rightarrow> 'a table" where
+fun trigger_results :: "\<I> \<Rightarrow> ts \<Rightarrow> 'a mtaux \<Rightarrow> 'a table" where
   "trigger_results I cur auxlist = {
     tuple.
+      (length (filter (\<lambda> (t, _, _). mem I (cur - t)) auxlist) > 0) \<and>
       \<comment> \<open>pretty much the definition of trigger\<close>
-      (\<exists>t relL relR. (t, relL, relR) \<in> (set auxlist) \<and> mem I (cur - t) \<and> 
+      (\<forall>i \<in> {0..<(length auxlist)}.
+        let (t, l, r) = auxlist!i in
+        mem I (cur - t) \<longrightarrow> 
         \<comment> \<open>either \<psi> holds or there is a later database where the same tuple satisfies \<phi>\<close>
-        (tuple \<in> relR \<or> (\<exists>t' relL' relR'. (t', relL', relR') \<in> (set auxlist) \<and> t < t' \<and> tuple \<in> relL'))
+        (
+          tuple \<in> r \<or>
+          (\<exists>j \<in> {i<..<(length auxlist)}.
+            let (t', l', r') = auxlist!j in
+            tuple \<in> l' \<comment> \<open>t < t' is given as the list is sorted\<close>
+          )
+        )
       )
 }"
 
@@ -70,42 +79,82 @@ type_synonym 'a mmtaux = "
   (ts \<times> 'a table \<times> 'a table) queue \<times>  \<comment> \<open>data_in: all databases containing the tuples satisfying the lhs or the rhs where the ts is in the interval\<close>
   (('a tuple, ts) mapping) \<times>           \<comment> \<open>tuple_in for once\<close>
   (('a tuple, ts) mapping) \<times>           \<comment> \<open>tuple_since for historically\<close>
-  (('a tuple, ts) mapping)             \<comment> \<open>tuple_since for \<psi> S (\<psi> \<and> \<phi>)\<close>
+  (('a tuple, ts) mapping) \<times>           \<comment> \<open>tuple_since for \<psi> S (\<psi> \<and> \<phi>)\<close>
+  ('a table)                            \<comment> \<open>the set of tuples currently satisfying trigger\<close>
 "
+
+fun time :: "(ts \<times> 'a table \<times> 'a table) \<Rightarrow> ts" where
+  "time db = fst db"
+
+fun relL :: "(ts \<times> 'a table \<times> 'a table) \<Rightarrow> 'a table" where
+  "relL db = (fst o snd) db"
+
+fun relR :: "(ts \<times> 'a table \<times> 'a table) \<Rightarrow> 'a table" where
+  "relR db = (snd o snd) db"
 
 definition ts_tuple_rel_binary :: "(ts \<times> 'a table \<times> 'a table) set \<Rightarrow> (ts \<times> 'a tuple \<times> 'a tuple) set" where
   "ts_tuple_rel_binary ys = {(t, as, bs). \<exists>X Y. as \<in> X \<and> bs \<in> Y \<and> (t, X, Y) \<in> ys}"
 
-definition valid_tuple :: "(('a tuple, ts) mapping) \<Rightarrow> (ts \<times> 'a tuple) \<Rightarrow> bool" where
-  "valid_tuple tuple_since = (\<lambda>(t, as). case Mapping.lookup tuple_since as of None \<Rightarrow> False
-  | Some t' \<Rightarrow> t \<ge> t')"
+definition ts_tuple_rel_binary_lhs :: "(ts \<times> 'a table \<times> 'a table) set \<Rightarrow> (ts \<times> 'a tuple) set" where
+  "ts_tuple_rel_binary_lhs ys = {(t, as). \<exists>X Y. as \<in> X \<and> (t, X, Y) \<in> ys}"
+
+definition ts_tuple_rel_binary_rhs :: "(ts \<times> 'a table \<times> 'a table) set \<Rightarrow> (ts \<times> 'a tuple) set" where
+  "ts_tuple_rel_binary_rhs ys = {(t, bs). \<exists>X Y. bs \<in> Y \<and> (t, X, Y) \<in> ys}"
 
 fun valid_mmtaux :: "targs \<Rightarrow> ts \<Rightarrow> 'a mmtaux \<Rightarrow> 'a mtaux \<Rightarrow> bool" where
-  "valid_mmtaux args cur (nt, maskL, maskR, data_prev, data_in, tuple_in_once, tuple_since_hist, tuple_since_since) ys \<longleftrightarrow>
-    (targs_L args) \<subseteq> (targs_R args) \<and>
+  "valid_mmtaux args cur (nt, maskL, maskR, data_prev, data_in, tuple_in_once, tuple_since_hist, tuple_since_since, sat) ys \<longleftrightarrow>
+    (if mem (targs_ivl args) 0 then (targs_L args) \<subseteq> (targs_R args) else (targs_L args) = (targs_R args)) \<and>
     maskL = join_mask (targs_n args) (targs_L args) \<and>
     maskR = join_mask (targs_n args) (targs_R args) \<and>
     (\<forall>(t, X, Y) \<in> set ys. table (targs_n args) (targs_R args) X \<and> table (targs_n args) (targs_L args) Y) \<and>
     table (targs_n args) (targs_R args) (Mapping.keys tuple_in_once) \<and>
     table (targs_n args) (targs_R args) (Mapping.keys tuple_since_hist) \<and>
     table (targs_n args) (targs_R args) (Mapping.keys tuple_since_since) \<and>
-    (\<forall>as \<in> \<Union>((fst o snd) ` (set (linearize data_prev))). wf_tuple (targs_n args) (targs_R args) as) \<and>
-    (\<forall>as \<in> \<Union>((snd o snd) ` (set (linearize data_prev))). wf_tuple (targs_n args) (targs_R args) as) \<and>
+    (\<forall>as \<in> \<Union>((relL) ` (set (linearize data_prev))). wf_tuple (targs_n args) (targs_R args) as) \<and>
+    (\<forall>as \<in> \<Union>((relR) ` (set (linearize data_prev))). wf_tuple (targs_n args) (targs_R args) as) \<and>
     cur = nt \<and>
-     \<comment> \<open>ts_tuple_rel_binary (set ys) =
-    {tas \<in> ts_tuple_rel_binary (set (linearize data_prev) \<union> set (linearize data_in)).
-    valid_tuple tuple_since tas} \<and>\<close>  \<comment> \<open>all tuples in data_prev and data_in have a (valid) entry in the mapping\<close>
-    sorted (map fst (linearize data_prev)) \<and>
+    \<comment> \<open>all valid lhs/\<phi> tuples in data_prev should have a valid entry in tuple_in_once, as it is shifted\<close>
+    ts_tuple_rel_binary_lhs (set (filter (\<lambda>(t, _, _). \<not>memL (targs_ivl args) t) ys)) =
+    {(t, l). \<exists>r. (t, l, r) \<in> ts_tuple_rel_binary (set (linearize data_prev)) \<and>
+    valid_tuple tuple_in_once (t, l)} \<and>
+    \<comment> \<open>all valid rhs/\<psi> tuples in data_in should have a valid entry in tuple_since_hist, as it is shifted\<close>
+    ts_tuple_rel_binary_rhs (set (filter (\<lambda>(t, _, _). mem (targs_ivl args) t) ys)) =
+    {(t, r). \<exists>l. (t, l, r) \<in> ts_tuple_rel_binary (set (linearize data_in)) \<and>
+    valid_tuple tuple_since_hist (t, r)} \<and>
+    \<comment> \<open>all valid \<phi>\<and>\<psi> tuples in data_in should have a valid entry in tuple_since_since, as it is shifted\<close>
+    ts_tuple_rel_binary (set (filter (\<lambda>(t, _, _). mem (targs_ivl args) t) ys)) =
+    {(t, l, r) \<in> ts_tuple_rel_binary (set (linearize data_in)).
+    valid_tuple tuple_since_since (t, l) \<and> valid_tuple tuple_since_since (t, r)} \<and>
+    \<comment> \<open>the entries stored should be the same, hence they're sorted as well\<close>
+    sorted (map fst ys) \<and>
+    ys = (linearize data_in) @ (linearize data_prev) \<and>
     (\<forall>t \<in> fst ` set (linearize data_prev). t \<le> nt \<and> \<not> memL (targs_ivl args) (nt - t)) \<and>
-    sorted (map fst (linearize data_in)) \<and>
-    (\<forall>t \<in> fst ` set (linearize data_in). t \<le> nt \<and> memL (targs_ivl args) (nt - t)) \<and>
-    valid_tuple_in ts_tuple_rel_binary data_in tuple_in (\<lambda>x. True) \<and>
+    (\<forall>t \<in> fst ` set (linearize data_in). t \<le> nt \<and> mem (targs_ivl args) (nt - t)) \<and>
+     \<comment> \<open>check whether tuple_in once contains the newest occurence of the tuple satisfying the lhs\<close>
+    newest_tuple_in_mapping ts_tuple_rel_binary_lhs data_in tuple_in_once (\<lambda>x. True) \<and>
     (\<forall>as \<in> Mapping.keys tuple_since_hist. case Mapping.lookup tuple_since_hist as of Some t \<Rightarrow> t \<le> nt) \<and>
-    (\<forall>as \<in> Mapping.keys tuple_since_since. case Mapping.lookup tuple_since_since as of Some t \<Rightarrow> t \<le> nt)
+    (\<forall>as \<in> Mapping.keys tuple_since_since. case Mapping.lookup tuple_since_since as of Some t \<Rightarrow> t \<le> nt) \<and>
+     \<comment> \<open>conditions for sat / trigger conditions\<close>
+    (\<forall>tuple. tuple \<in> sat \<longleftrightarrow>
+      (set (linearize data_in) \<noteq> {}) \<and> ( \<comment> \<open>with an empty data_in, all tuples satisfy trigger\<close>
+        (\<forall>i \<in> {0..<(length (linearize data_in))}.
+          let (t, l, r) = (linearize data_in)!i in
+          tuple \<in> r \<or>
+          (\<exists>j \<in> {i<..<(length (linearize data_in))}.
+            let (t', l', r') = (linearize data_in)!j in
+            tuple \<in> l'
+          )
+        ) \<or>
+        (\<exists>(t, l, r) \<in> set (linearize data_prev).
+          tuple \<in> l
+        )
+      )
+    )
   "
 
-fun init_mmtaux :: "targs \<Rightarrow> event_data mmtaux" where
-  "init_mmtaux args = (0, [], [], empty_queue, empty_queue, Mapping.empty, Mapping.empty, Mapping.empty)"
+definition init_mmtaux :: "targs \<Rightarrow> 'a mmtaux" where
+  "init_mmtaux args = (0, join_mask (targs_n args) (targs_L args),
+  join_mask (targs_n args) (targs_R args), empty_queue, empty_queue, Mapping.empty, Mapping.empty, Mapping.empty, {})"
 
 lemma valid_init_mtaux: "(
     if (mem I 0)
@@ -114,21 +163,601 @@ lemma valid_init_mtaux: "(
       else 
         L = R
     ) \<Longrightarrow>
+    let args = init_targs I n L R in
     valid_mmtaux args 0 (init_mmtaux args) []"
-  by (auto simp add: trigger_results_def)
+  unfolding init_mmtaux_def
+  by (auto simp add: init_targs_def empty_queue_rep
+      Mapping.lookup_empty safe_max_def table_def newest_tuple_in_mapping_def
+      ts_tuple_rel_binary_def ts_tuple_rel_binary_lhs_def ts_tuple_rel_binary_rhs_def)
 
+(* analogous to add_new_ts_mmsaux' *)
+fun add_new_ts_mmtaux' :: "args \<Rightarrow> ts \<Rightarrow> 'a mmtaux \<Rightarrow> 'a mmtaux" where
+  "add_new_ts_mmtaux' args nt (t, maskL, maskR, data_prev, data_in, tuple_in_once, tuple_since_hist, tuple_since_since, sat) = (
+    let I = args_ivl args;
+     \<comment> \<open>split into the part that still is data_prev and the dbs that are no longer before I\<close>
+    (data_prev, move) = takedropWhile_queue (\<lambda>(t, _). memL I (nt - t)) data_prev;
+     \<comment> \<open>next the data from data_prev that is larger than the lower boundary is appended to data_in\<close>
+    data_in = fold (\<lambda>(t, X) data_in. append_queue (t, X) data_in) move data_in;
+    \<comment> \<open>next the data from data_prev that is larger than the lower boundary is appended to data_in\<close>
+    (data_in, drop) = takedropWhile_queue (\<lambda>(t, _). memR I (nt - t)) data_in
+    in
+    (
+      nt,                  \<comment> \<open>update ts\<close>
+      maskL,               \<comment> \<open>keep masks\<close>
+      maskR,
+      data_prev,           \<comment> \<open>updated according to I\<close>
+      data_in,             \<comment> \<open>updated according to I\<close>
+      tuple_in_once,       \<comment> \<open>kept as we only do operations regarding the new ts here and 
+                              this mapping should only be updated for the new db\<close>
+      tuple_since_hist,    \<comment> \<open>kept as\<close>
+      tuple_since_since,
+      sat
+    )
+  )"
+
+
+fun update_mmtaux :: "targs \<Rightarrow> ts \<Rightarrow> event_data table \<Rightarrow> event_data table \<Rightarrow> 'a mmtaux \<Rightarrow> 'a mmtaux" where
+  "update_mmtaux args nt l r (cur, maskL, maskR, data_prev, data_in, tuple_in_once, tuple_since_hist, tuple_since_since, sat) =
+
+
+  (
+    nt,
+    maskL,
+    maskR,
+    data_prev,
+    data_in,
+    tuple_in_once,
+    tuple_since_hist,
+    tuple_since_since,
+    sat
+  )"
 
 fun result_mmtaux :: "targs \<Rightarrow> event_data mmtaux \<Rightarrow> event_data table" where
-  "result_mmtaux args (nt, maskL, maskR, data_prev, data_in, tuple_in_once, tuple_since_hist, tuple_since_since) = 
-  {}
+  "result_mmtaux args (nt, maskL, maskR, data_prev, data_in, tuple_in_once, tuple_since_hist, tuple_since_since, sat) = 
+  sat
 "
 
-(* tail recursive function to split a list into two based on a predicate while maintaining the order *)
-fun split_list :: "('a \<Rightarrow> bool) \<Rightarrow> 'a list \<Rightarrow> 'a list \<Rightarrow> 'a list \<Rightarrow> 'a list \<times> 'a list" where
-  "split_list p [] t f = (t, f)"
-| "split_list p (x#xs) t f = (if (p x) then split_list p xs (x#t) f else split_list p xs t (x#f))"
+lemma data_in_mem:
+  assumes "valid_mmtaux args cur (nt, maskL, maskR, data_prev, data_in, tuple_in_once, tuple_since_hist, tuple_since_since, sat) auxlist"
+  assumes "db \<in> set (linearize data_in)"
+  shows "mem (targs_ivl args) (nt - (time db))"
+  using assms by auto
 
+lemma data_prev_mem:
+  assumes "valid_mmtaux args cur (nt, maskL, maskR, data_prev, data_in, tuple_in_once, tuple_since_hist, tuple_since_since, sat) auxlist"
+  assumes "db \<in> set (linearize data_prev)"
+  shows "\<not>memL (targs_ivl args) (nt - (time db))"
+  using assms by auto
 
+lemma auxlist_mem_data_in:
+  assumes "valid_mmtaux args cur (nt, maskL, maskR, data_prev, data_in, tuple_in_once, tuple_since_hist, tuple_since_since, sat) auxlist"
+  assumes "db \<in> (set auxlist)"
+  assumes "mem (targs_ivl args) (nt - (time db))"
+  shows "db \<in> set (linearize data_in)"
+proof -
+  have "db \<in> set (linearize data_in) \<or> db \<in> set (linearize data_prev)"
+    using assms by auto
+  moreover have "db \<in> set (linearize data_prev) \<Longrightarrow> False"
+  using data_prev_mem[OF assms(1)] assms(3)
+    by auto
+  ultimately have "db \<in> set (linearize data_in)" by auto
+  then show ?thesis by blast
+qed
+
+lemma data_sorted:
+  assumes "valid_mmtaux args cur (nt, maskL, maskR, data_prev, data_in, tuple_in_once, tuple_since_hist, tuple_since_since, sat) auxlist"
+  shows "sorted (map fst (linearize data_prev))" "sorted (map fst (linearize data_in))"
+proof -
+  from assms have "sorted (map fst auxlist)"
+    by auto
+  moreover from assms have "auxlist = (linearize data_in) @ (linearize data_prev)"
+    by auto
+  ultimately show "sorted (map fst (linearize data_prev))" "sorted (map fst (linearize data_in))"
+    using sorted_append by auto
+qed
+
+lemma auxlist_index_time_mono:
+  assumes "valid_mmtaux args cur (nt, maskL, maskR, data_prev, data_in, tuple_in_once, tuple_since_hist, tuple_since_since, sat) auxlist"
+  assumes "i \<le> j" "j \<in> {0..<(length auxlist)}"
+  shows "fst (auxlist!i) \<le> fst (auxlist!j)"
+proof -
+  from assms have "sorted (map fst auxlist)" by auto
+  then have sorted: "\<forall>i. \<forall>j \<in> {0..<(length auxlist)}.
+    i \<le> j \<longrightarrow> fst (auxlist!i) \<le> fst (auxlist!j)"
+    by (simp add: sorted_iff_nth_mono)
+  then show "fst (auxlist!i) \<le> fst (auxlist!j)"
+    using sorted assms(2-3)
+    by auto
+qed
+
+lemma auxlist_time_index_strict_mono:
+  assumes "valid_mmtaux args cur (nt, maskL, maskR, data_prev, data_in, tuple_in_once, tuple_since_hist, tuple_since_since, sat) auxlist"
+  assumes "i \<in> {0..<(length auxlist)}"
+  assumes "fst (auxlist!i) < fst (auxlist!j)" (* t < t' *)
+  shows "i < j"
+proof -
+    {
+      assume assm: "j \<le> i"
+      then have "False"
+        using auxlist_index_time_mono[OF assms(1) assm assms(2)] assms(3)
+        by auto
+    }
+    then show "i < j" using le_def by blast
+  qed
+
+lemma data_prev_auxlist_index:
+  assumes "valid_mmtaux args cur (nt, maskL, maskR, data_prev, data_in, tuple_in_once, tuple_since_hist, tuple_since_since, sat) auxlist"
+  assumes "i \<in> {0..<(length (linearize data_prev))}"
+  shows "auxlist!((length (linearize data_in)) + i) = (linearize data_prev)!i" "(length (linearize data_in)) + i < (length auxlist)"
+proof -
+  from assms(1) have "auxlist = (linearize data_in) @ (linearize data_prev)" by auto
+  then show "auxlist!((length (linearize data_in)) + i) = (linearize data_prev)!i"
+    using nth_append_length_plus
+    by blast
+next
+  from assms(1) have "auxlist = (linearize data_in) @ (linearize data_prev)" by auto
+  then show "(length (linearize data_in)) + i < (length auxlist)" using assms(2) by auto
+qed
+
+lemma data_prev_auxlist_index_rev:
+  assumes "valid_mmtaux args cur (nt, maskL, maskR, data_prev, data_in, tuple_in_once, tuple_since_hist, tuple_since_since, sat) auxlist"
+  assumes "i \<in> {(length (linearize data_in))..<(length auxlist)}"
+  shows "auxlist!i = (linearize data_prev)!(i - (length (linearize data_in)))"
+        "i - (length (linearize data_in)) < (length (linearize data_prev))"
+proof -
+  from assms(1) have "auxlist = (linearize data_in) @ (linearize data_prev)" by auto
+  then show "auxlist!i = (linearize data_prev)!(i - (length (linearize data_in)))"
+    using assms(2)
+  by (simp add: nth_append)
+next
+  from assms(1) have "auxlist = (linearize data_in) @ (linearize data_prev)" by auto
+  then show "i - (length (linearize data_in)) < (length (linearize data_prev))"
+    using assms(2)
+    by auto
+qed
+
+lemma data_prev_set_mem:
+  assumes "valid_mmtaux args cur (nt, maskL, maskR, data_prev, data_in, tuple_in_once, tuple_since_hist, tuple_since_since, sat) auxlist"
+  assumes "i \<in> {(length (linearize data_in))..<(length auxlist)}"
+  shows "auxlist!i \<in> set (linearize data_prev)"
+proof - 
+  have "auxlist!i = (linearize data_prev)!(i - (length (linearize data_in)))"
+       "i - (length (linearize data_in)) < (length (linearize data_prev))"
+    using data_prev_auxlist_index_rev[OF assms(1) assms(2)] by auto
+  then show ?thesis by simp
+qed
+
+lemma data_in_auxlist_index:
+  assumes "valid_mmtaux args cur (nt, maskL, maskR, data_prev, data_in, tuple_in_once, tuple_since_hist, tuple_since_since, sat) auxlist"
+  assumes "i \<in> {0..<(length (linearize data_in))}"
+  shows "auxlist!i = (linearize data_in)!i" "i < length (auxlist)" "auxlist!i \<in> set (linearize data_in)"
+proof -
+  from assms(1) have "auxlist = (linearize data_in) @ (linearize data_prev)" by auto
+  then show "auxlist!i = (linearize data_in)!i" "i < length (auxlist)" "auxlist!i \<in> set (linearize data_in)"
+    using nth_append[of "(linearize data_in)" "(linearize data_prev)" i] assms(2)
+    by auto
+qed
+
+lemma data_in_auxlist_nonempty:
+  assumes "valid_mmtaux args cur (nt, maskL, maskR, data_prev, data_in, tuple_in_once, tuple_since_hist, tuple_since_since, sat) auxlist"
+  shows "(length (filter (\<lambda> (t, _, _). mem (targs_ivl args) (nt - t)) auxlist) > 0) = (set (linearize data_in) \<noteq> {})"
+proof (rule iffI)
+  assume assm: "length (filter (\<lambda> (t, _, _). mem (targs_ivl args) (nt - t)) auxlist) > 0"
+  {
+    assume empty: "set (filter (\<lambda> (t, _, _). mem (targs_ivl args) (nt - t)) auxlist) = {}"
+    {
+      assume "length (filter (\<lambda> (t, _, _). mem (targs_ivl args) (nt - t)) auxlist) > 0"
+      then have "\<exists>x. x \<in> set (filter (\<lambda> (t, _, _). mem (targs_ivl args) (nt - t)) auxlist)"
+        using nth_mem by blast
+      then have "False" using empty by auto
+    }
+    then have "length (filter (\<lambda> (t, _, _). mem (targs_ivl args) (nt - t)) auxlist) = 0"
+      by auto
+    then have "False" using assm by auto
+  }
+  then obtain db where db_props: "db \<in> set (filter (\<lambda> (t, _, _). mem (targs_ivl args) (nt - t)) auxlist)"
+    by auto
+  then have "db \<in> set auxlist" "mem (targs_ivl args) (nt - fst db)" by auto
+  then have "db \<in> set (linearize data_in)" using auxlist_mem_data_in[OF assms(1)] by auto
+  then show "set (linearize data_in) \<noteq> {}" by auto
+  next
+    assume "set (linearize data_in) \<noteq> {}"
+    then obtain db where db_props: "db \<in> set (linearize data_in)" by (meson nonemptyE)
+    then have db_mem: "db \<in> set auxlist" using assms(1) by auto
+    then have "mem (targs_ivl args) (nt - fst db)"
+      using data_in_mem[OF assms(1)] db_props
+      by auto
+    then have "db \<in> set (filter (\<lambda> (t, _, _). mem (targs_ivl args) (nt - t)) auxlist)"
+      using db_mem
+      by auto
+    then show auxlist_nonempty: "(length (filter (\<lambda> (t, _, _). mem (targs_ivl args) (nt - t)) auxlist) > 0)"
+      using length_pos_if_in_set[of db "filter (\<lambda> (t, _, _). mem (targs_ivl args) (nt - t)) auxlist"]
+      by auto
+qed
+
+(*lemma data_prev_auxlist_index:
+  assumes "valid_mmtaux args cur (nt, maskL, maskR, data_prev, data_in, tuple_in_once, tuple_since_hist, tuple_since_since, sat) auxlist"
+  assumes "i \<in> {length (linearize data_prev)..<(length auxlist)}"
+  shows "auxlist!i = (linearize data_in)!(i - length (linearize data_prev))"
+proof -
+  from assms(1) have "auxlist = (linearize data_prev) @ (linearize data_in)" by auto
+  then show ?thesis using assms(2) by (simp add: nth_append)
+qed*)
+
+lemma valid_result_mmtaux: 
+  assumes "valid_mmtaux args cur (nt, maskL, maskR, data_prev, data_in, tuple_in_once, tuple_since_hist, tuple_since_since, sat) auxlist"
+  shows "result_mmtaux args (nt, maskL, maskR, data_prev, data_in, tuple_in_once, tuple_since_hist, tuple_since_since, sat) = trigger_results (targs_ivl args) cur auxlist"
+proof -
+  define aux where "aux = (nt, maskL, maskR, data_prev, data_in, tuple_in_once, tuple_since_hist, tuple_since_since, sat)"
+  define I where "I = targs_ivl args"
+  from assms(1) have time: "nt = cur" by auto
+  {
+    fix tuple
+    assume "tuple \<in> result_mmtaux args aux"
+    then have mem_sat: "tuple \<in> sat" using aux_def by auto
+    then have "set (linearize data_in) \<noteq> {}" using assms(1) by auto
+    then have auxlist_nonempty: "(length (filter (\<lambda> (t, _, _). mem I (nt - t)) auxlist) > 0)"
+      using data_in_auxlist_nonempty[OF assms(1)] I_def
+      by auto
+    then have "(\<forall>i \<in> {0..<(length (linearize data_in))}.
+        let (t, l, r) = (linearize data_in)!i in
+        tuple \<in> r \<or>
+        (\<exists>j \<in> {i<..<(length (linearize data_in))}.
+          let (t', l', r') = (linearize data_in)!j in
+          tuple \<in> l'
+        )
+      ) \<or>
+      (\<exists>(t, l, r) \<in> set (linearize data_prev).
+        tuple \<in> l
+      )" using mem_sat assms
+      by auto
+    moreover {
+      assume "\<exists>(t, l, r) \<in> set (linearize data_prev). tuple \<in> l"
+      then obtain t l r where 
+          db_props: "(t, l, r) \<in> set (linearize data_prev)"
+          "tuple \<in> l"
+        by blast
+      then have "\<not>memL I (nt - t)"
+        using I_def data_prev_mem[OF assms(1)]
+        by auto
+      then have int: "\<forall>t'. mem I (nt - t') \<longrightarrow> t' < t"
+        by (meson diff_le_mono2 leI memL_mono)
+      have auxlist_mem: "(t, l, r) \<in> set auxlist"
+        using db_props assms
+        by auto
+      then obtain j where j_props: "(t, l, r) = auxlist!j" "j <(length auxlist)"
+        using in_set_conv_nth[of "(t, l, r)" auxlist] by force
+      then have t_props: "t = fst ((auxlist)!j)"
+        by (metis eq_fst_iff)
+      {
+        fix i
+        assume i_props: "i \<in> {0..<(length auxlist)}"
+        define dbi where "dbi = auxlist!i"
+        define t' where "t' = fst dbi"
+        define l' where "l' = relL dbi"
+        define r' where "r' = relR dbi"
+        assume "mem I (nt - t')"
+        then have "t' < t" using int by auto
+        then have "i < j"
+          using auxlist_time_index_strict_mono[OF assms(1) i_props] dbi_def t'_def t_props
+          by auto
+        then have "(\<exists>j \<in> {i<..<(length auxlist)}.
+          let (t', l', r') = auxlist!j in
+          tuple \<in> l'
+        )" using i_props j_props db_props(2) by force
+      }
+      then have "(\<forall>i \<in> {0..<(length auxlist)}.
+        let (t, l, r) = auxlist!i in
+        mem I (nt - t) \<longrightarrow> (\<exists>j \<in> {i<..<(length auxlist)}.
+          let (t', l', r') = auxlist!j in
+          tuple \<in> l'
+        )
+      )" by auto
+      then have "tuple \<in> trigger_results I nt auxlist"
+        using auxlist_nonempty
+        by auto
+    }
+    moreover {
+      assume assm: "(\<forall>i \<in> {0..<(length (linearize data_in))}.
+        let (t, l, r) = (linearize data_in)!i in
+        tuple \<in> r \<or>
+        (\<exists>j \<in> {i<..<(length (linearize data_in))}.
+          let (t', l', r') = (linearize data_in)!j in
+          tuple \<in> l'
+        )
+      )"
+      {
+        assume hist: "\<forall>i \<in> {0..<(length (linearize data_in))}.
+        let (t, l, r) = (linearize data_in)!i in
+        tuple \<in> r"
+        {
+          fix i
+          define dbi where "dbi = auxlist!i"
+          define t where "t = time dbi"
+          define l where "l = relL dbi"
+          define r where "r = relR dbi"
+          assume i_props: "i \<in> {0..<(length auxlist)}" "mem I (nt - t)"
+          {
+            assume "i \<ge> (length (linearize data_in))"
+            then have "dbi \<in> set (linearize data_prev)"
+              using data_prev_set_mem[OF assms(1)] i_props dbi_def
+              by auto
+            then have "\<not>memL I (nt - t)"
+              using data_prev_mem[OF assms(1)] t_def I_def
+              by auto
+          }
+          then have i_le: "i < (length (linearize data_in))" using i_props(2) le_def by blast
+          moreover have "(linearize data_in)!i = auxlist!i"
+            using i_le data_in_auxlist_index[OF assms(1)]
+            by auto
+          ultimately have
+            "i \<in> {0..<(length (linearize data_in))}"
+            "(t, l, r) = (linearize data_in)!i"
+            using t_def l_def r_def dbi_def
+            by auto
+          then have "tuple \<in> r" using hist by fastforce
+        }
+        then have "\<forall>i \<in> {0..<(length auxlist)}.
+        let (t, l, r) = auxlist!i in
+        mem I (nt - t) \<longrightarrow> tuple \<in> r"
+          by (simp add: case_prod_beta')
+        then have "tuple \<in> trigger_results I nt auxlist"
+          using auxlist_nonempty
+          by auto
+      }
+      moreover {
+        define A where "A = {i \<in> {0..<(length (linearize data_in))}. tuple \<notin> relR ((linearize data_in)!i)}"
+        define i where "i = Max A"
+        assume "\<not>(\<forall>i \<in> {0..<(length (linearize data_in))}.
+        let (t, l, r) = (linearize data_in)!i in
+        tuple \<in> r)"
+        then have A_props: "A \<noteq> {}" "finite A" using A_def by auto
+        then have "i \<in> A" using i_def by auto
+        then have i_props:
+          "i \<in> {0..<(length (linearize data_in))}"
+          "tuple \<notin> relR ((linearize data_in)!i)"
+          using A_def
+          by auto
+        then obtain j where j_props:
+          "j \<in> {i<..<(length (linearize data_in))}"
+          "let (t', l', r') = (linearize data_in)!j in
+          tuple \<in> l'"
+          using assm
+          by fastforce
+        then have j_idx:
+          "(linearize data_in)!j = auxlist!j"
+          "j < (length auxlist)"
+          using data_in_auxlist_index[OF assms(1)]
+          by auto
+        {
+          fix k
+          define dbk where "dbk = auxlist!k"
+          define t_k where "t_k = time dbk"
+          define l_k where "l_k = relL dbk"
+          define r_k where "r_k = relR dbk"
+          assume k_props: "k \<in> {0..<(length auxlist)}" "mem I (nt - t_k)"
+          {
+            assume "k \<ge> (length (linearize data_in))"
+            then have "dbk \<in> set (linearize data_prev)"
+              using data_prev_set_mem[OF assms(1)] k_props dbk_def
+              by auto
+            then have "\<not>memL I (nt - t_k)"
+              using data_prev_mem[OF assms(1)] t_k_def I_def
+              by auto
+          }
+          then have k_le: "k < (length (linearize data_in))" using k_props(2) le_def by blast
+          then have k_idx: "(linearize data_in)!k = auxlist!k"
+            using data_in_auxlist_index[OF assms(1)]
+            by auto
+          {
+            assume "tuple \<notin> r_k"
+            then have "k \<in> A" using k_le A_def r_k_def dbk_def k_idx by auto
+            then have "k \<le> i" using i_def A_props by auto
+            then have "j \<in> {k<..<(length auxlist)}"
+              "let (t', l', r') = auxlist!j in
+              tuple \<in> l'"
+              using j_props j_idx
+              by auto
+            then have "\<exists>j \<in> {k<..<(length auxlist)}.
+              let (t', l', r') = auxlist!j in
+              tuple \<in> l'"
+              by blast
+          }
+          then have "tuple \<in> r_k \<or>
+          (\<exists>j \<in> {k<..<(length auxlist)}.
+            let (t', l', r') = auxlist!j in
+            tuple \<in> l'
+          )" by blast
+        }
+        then have "\<forall>i \<in> {0..<(length auxlist)}.
+          mem I (nt - time (auxlist!i)) \<longrightarrow> 
+          (
+            tuple \<in> relR (auxlist!i) \<or>
+            (\<exists>j \<in> {i<..<(length auxlist)}.
+              let (t', l', r') = auxlist!j in
+              tuple \<in> l'
+            )
+          )"
+          by auto
+        then have "tuple \<in> trigger_results I nt auxlist"
+          using auxlist_nonempty
+          by auto
+      }
+      ultimately have "tuple \<in> trigger_results I nt auxlist"
+        by blast
+    }
+    ultimately have "tuple \<in> trigger_results I nt auxlist" by blast
+    then have "tuple \<in> trigger_results (targs_ivl args) cur auxlist"
+      using I_def time
+      by auto
+  }
+  then have subset: "result_mmtaux args aux \<subseteq> trigger_results (targs_ivl args) cur auxlist"
+    by blast
+  {
+    fix tuple
+    assume "tuple \<in> trigger_results (targs_ivl args) cur auxlist"
+    then have el: "tuple \<in> trigger_results I cur auxlist"
+      by (simp add: I_def)
+    then have data_in_nonempty: "(set (linearize data_in) \<noteq> {})"
+      using data_in_auxlist_nonempty[OF assms(1)] I_def time
+      by auto
+    from el have trigger: "(\<forall>i \<in> {0..<(length auxlist)}.
+        let (t, l, r) = auxlist!i in
+        mem I (cur - t) \<longrightarrow> 
+        (
+          tuple \<in> r \<or>
+          (\<exists>j \<in> {i<..<(length auxlist)}.
+            let (t', l', r') = auxlist!j in
+            tuple \<in> l'
+          )
+        )
+      )" by auto
+    {
+      (* historically *)
+      assume hist: "\<forall>i \<in> {0..<(length auxlist)}.
+        let (t, l, r) = auxlist!i in
+        mem I (cur - t) \<longrightarrow> tuple \<in> r"
+      {
+        fix i
+        define dbi where "dbi = (linearize data_in)!i"
+        assume i_props: "i \<in> {0..<(length (linearize data_in))}"
+        then have i_props:
+          "dbi \<in> set (linearize data_in)"
+          "i < length auxlist"
+          "auxlist ! i = linearize data_in ! i"
+          using data_in_auxlist_index[OF assms(1) i_props] dbi_def
+          by auto
+        then have "mem I (cur - time dbi)"
+          using data_in_mem[OF assms(1)] dbi_def I_def time
+          by auto
+        then have "tuple \<in> relR dbi"
+          using hist dbi_def i_props
+          by (smt atLeastLessThan_iff case_prod_beta' comp_apply relR.simps time.simps zero_le)
+      }
+      then have "(\<forall>i \<in> {0..<(length (linearize data_in))}.
+          let (t, l, r) = (linearize data_in)!i in
+          tuple \<in> r
+        )"
+        by fastforce
+      then have "tuple \<in> sat"
+        using assms(1) data_in_nonempty
+        by auto
+    }
+    moreover {
+      define A where "A = {i \<in> {0..<(length auxlist)}. mem I (cur - time (auxlist!i)) \<and> tuple \<notin> relR (auxlist!i)}"
+      define i where "i = Max A"
+      assume "\<not>(\<forall>i \<in> {0..<(length auxlist)}.
+        let (t, l, r) = auxlist!i in
+        mem I (cur - t) \<longrightarrow> tuple \<in> r)"
+      then have "\<not>(\<forall>i \<in> {0..<(length auxlist)}.
+        mem I (cur - time (auxlist!i)) \<longrightarrow> tuple \<in> relR (auxlist!i))"
+        by fastforce
+      then have A_props: "A \<noteq> {}" "finite A" using A_def by auto
+      then have "i \<in> A" using i_def by auto
+      then have i_props:
+        "i \<in> {0..<(length auxlist)}"
+        "mem I (cur - time (auxlist!i))"
+        "tuple \<notin> relR (auxlist!i)"
+        using A_def
+        by auto
+      then have "(\<exists>j \<in> {i<..<(length auxlist)}.
+        let (t', l', r') = auxlist!j in
+        tuple \<in> l'
+      )"
+        using trigger
+        by fastforce
+      then obtain j where j_props:
+        "j \<in> {i<..<(length auxlist)}"
+        "let (t', l', r') = auxlist!j in
+        tuple \<in> l'"
+        by auto
+      {
+        (* \<phi> in data_prev *)
+        define j' where "j' = (j - length (linearize data_in))"
+        assume assm: "j \<ge> (length (linearize data_in))"
+        then have j'_props:
+          "auxlist!j = linearize data_prev!j'"
+          "j' < length (linearize data_prev)"
+          using data_prev_auxlist_index_rev[OF assms(1)] j_props(1) j'_def
+          by auto
+        then have "auxlist!j \<in> set (linearize data_prev)"
+          using j_props assm nth_mem
+          by fastforce
+        then have "\<exists>(t, l, r) \<in> set (linearize data_prev). tuple \<in> l"
+          using j_props(2)
+          by meson
+        then have "tuple \<in> sat"
+          using data_in_nonempty assms(1)
+          by auto
+      }
+      moreover {
+        (* \<psi> S \<psi> \<and> \<phi> in data_in *)
+        assume j_le: "j < (length (linearize data_in))"
+        then have j_idx:
+          "(linearize data_in)!j = auxlist!j"
+          "j < length auxlist"
+          "auxlist ! j \<in> set (linearize data_in)"
+          using data_in_auxlist_index[OF assms(1)] j_props
+          by auto
+        {
+          fix k
+          define db where "db = (linearize data_in)!k"
+          define r where "r = relR db"
+          assume k_props: "k \<in> {0..<(length (linearize data_in))}"
+          then have k_idx:
+            "(linearize data_in)!k = auxlist!k"
+            "k < length auxlist"
+            "auxlist ! k \<in> set (linearize data_in)"
+            using data_in_auxlist_index[OF assms(1)]
+            by auto
+          then have k_mem: "mem I (nt - time (auxlist!k))"
+            using data_in_mem[OF assms(1) k_idx(3)] I_def
+            by auto
+          {
+            assume "tuple \<notin> r"
+            then have "k \<in> A" using A_def k_idx k_mem time r_def db_def by auto
+            then have "k \<le> i" using i_def A_props by auto
+            then have "j \<in> {k<..<(length (linearize data_in))}"
+            "let (t', l', r') = (linearize data_in)!j in
+            tuple \<in> l'"
+              using j_le j_props j_idx
+              by auto
+            then have "\<exists>j \<in> {k<..<(length (linearize data_in))}.
+            let (t', l', r') = (linearize data_in)!j in
+            tuple \<in> l'"
+              by fastforce
+          }
+          then have "tuple \<in> r \<or>
+          (\<exists>j \<in> {k<..<(length (linearize data_in))}.
+            let (t', l', r') = (linearize data_in)!j in
+            tuple \<in> l'
+          )" by blast
+        }
+        then have "(\<forall>i \<in> {0..<(length (linearize data_in))}.
+          let (t, l, r) = (linearize data_in)!i in
+          tuple \<in> r \<or>
+          (\<exists>j \<in> {i<..<(length (linearize data_in))}.
+            let (t', l', r') = (linearize data_in)!j in
+            tuple \<in> l'
+          )
+        )"
+          by (simp add: case_prod_beta')
+        then have "tuple \<in> sat"
+          using data_in_nonempty assms(1)
+          by auto
+      }
+      ultimately have "tuple \<in> sat" using not_le by blast
+    }
+    ultimately have "tuple \<in> sat" by blast
+    then have "tuple \<in> result_mmtaux args aux" using aux_def by auto
+  }
+  then have "trigger_results (targs_ivl args) cur auxlist \<subseteq> result_mmtaux args aux"
+    by auto
+  then have "trigger_results (targs_ivl args) cur auxlist = result_mmtaux args aux"
+    using subset
+    by blast
+  then show ?thesis using aux_def by auto
+qed
 
 
 (*
